Prove "skeleton" of heaplang adequacy theorem.

src/heaplang/adequacy.v
@@ -8,7 +8,13 @@ From iris.itree.threadpool Require Import handler.
 From iris.itree.heaplang Require Import lang.
 Context {Σ} `{!invGS_gen hlc Σ} `{!heaplangHGS Σ}.
 
+Lemma compile_Fork_value {R} e (k : val → itree heaplangE R) :
+  is_value e = true →
+  (v ← compile_expr (Fork e) ; k v)%itree ≈ k (LitV LitUnit).
+Admitted.
+
 Lemma compile_Fork {R} e (k : val → itree heaplangE R) :
+  is_value e = false →
   (v ← compile_expr (Fork e) ; k v)%itree ≈ vis EFork (λ thread,
     match thread with
     | CurrentThread => k (LitV LitUnit)
@@ -18,7 +24,8 @@ Lemma compile_Fork {R} e (k : val → itree heaplangE R) :
     end
   )%itree.
 Proof.
-  rewrite /compile_expr !rec_as_interp interp_bind.
+  intros Hval.
+  rewrite /compile_expr !rec_as_interp /= Hval interp_bind.
   setoid_rewrite interp_trigger. simpl.
   rewrite -bind_trigger bind_bind. f_equiv. intros [|].
   - rewrite interp_ret bind_ret_l //.
@@ -28,11 +35,12 @@ Proof.
 Qed.
 
 Lemma trace_base_Fork {R} tid (tp : list (itree heaplangE R)) tr e k :
+  is_value e = false →
   tp !! tid = Some (v ← compile_expr (Fork e) ; k v)%itree →
   is_ctrace tr tid (<[tid := k (LitV LitUnit)]>tp ++ [(compile_expr e ;; kill_thread)%itree]) →
   is_ctrace (CTFork (compile_expr e ;; kill_thread) tr) tid tp.
 Proof.
-  intros Htp Htr. eapply is_ctrace_insert; first done; first apply compile_Fork; eauto.
+  intros Hval Htp Htr. eapply is_ctrace_insert; first done; first apply compile_Fork; eauto.
   eexists. split. { rewrite list_lookup_insert //. by apply lookup_lt_is_Some_1. }
   constructor.
   rewrite /compile_expr rec_as_interp //. rewrite list_insert_insert.
@@ -67,10 +75,30 @@ Proof.
   - setoid_rewrite interp_trigger. f_equiv; first done. by intros _.
 Qed.
 
-Lemma step_in_thread {R} e1 σ1 κs e2 σ2 efs tr tid tid' tp (k : val → itree heaplangE R) :
+Definition compile_tp (tp : list expr) : list (itree heaplangE ()) :=
+  map (λ e, compile_expr e ;; kill_thread)%itree (List.filter (λ e, negb (is_value e)) tp).
+
+Lemma compile_tp_app (tp tp' : list expr) :
+  compile_tp (tp ++ tp') = compile_tp tp ++ compile_tp tp'.
+Admitted.
+
+Lemma compile_tp_cons (e : expr) (tp : list expr) :
+  compile_tp (e :: tp) = if is_value e then compile_tp tp else (compile_expr e ;; kill_thread)%itree :: compile_tp tp.
+Admitted.
+
+Lemma compile_tp_empty (tp : list expr) :
+  Forall is_value tp →
+  compile_tp tp = [].
+Admitted.
+Lemma compile_tp_empty_inv (tp : list expr) :
+  compile_tp tp = [] →
+  Forall is_value tp.
+Admitted.
+
+Lemma step_in_thread e1 σ1 κs e2 σ2 efs tr tid tid' tp (k : val → itree heaplangE ()) :
   base_step e1 σ1 κs e2 σ2 efs →
   is_ctrace tr tid' (<[tid:=(v ← compile_expr e2 ; yield_if_not_val e2 ;; k v)%itree]>tp
-                    ++ map (λ e, compile_expr e ;; kill_thread)%itree efs) →
+                    ++ compile_tp efs) →
   tp !! tid = Some (v ← compile_expr e1 ; yield_if_not_val e1 ;; k v)%itree →
   ∃ tr', is_postfix tr tr' ∧ is_ctrace tr' tid tp.
 Proof.
@@ -92,7 +120,7 @@ Proof.
       rewrite compile_expr_val. rewrite compile_expr_val in Htr.
       simpl in Htr.
       rewrite bind_ret_l. rewrite !bind_ret_l in Htr.
-      apply ctrace_yield with (t := k v).
+      apply is_ctrace_yield with (t := k v).
       { rewrite list_lookup_insert //. by apply lookup_lt_is_Some. }
       by rewrite list_insert_insert.
     * eapply is_ctrace_insert; first done.
@@ -100,7 +128,7 @@ Proof.
         rewrite Hval. reflexivity. }
       rewrite /e' in Hval. rewrite /yield_if_not_val in Htr. rewrite Hval in Htr.
       rewrite bind_bind.
-      apply ctrace_yield with (t := (v ← compile_expr e'; trigger EYield ;; k v)%itree).
+      apply is_ctrace_yield with (t := (v ← compile_expr e'; trigger EYield ;; k v)%itree).
       { rewrite list_lookup_insert //. by apply lookup_lt_is_Some. }
       by rewrite list_insert_insert.
   - admit.
@@ -108,7 +136,7 @@ Proof.
     rewrite compile_expr_val !bind_ret_l in Htr.
     eapply is_ctrace_insert with (t' := (trigger EYield ;; k v')%itree); first done.
     { rewrite base_BinOp // bind_ret_l  //. }
-    eapply ctrace_yield. { rewrite list_lookup_insert //. by apply lookup_lt_is_Some. }
+    eapply is_ctrace_yield. { rewrite list_lookup_insert //. by apply lookup_lt_is_Some. }
     by rewrite list_insert_insert.
   - admit.
   - admit.
@@ -123,49 +151,148 @@ Proof.
   - admit.
   - admit.
   - admit.
-  - exists (CTFork (compile_expr e ;; kill_thread) (CTYield tid' tr)).
-    split; first repeat constructor.
-    rewrite compile_expr_val !bind_ret_l in Htr.
-    eapply trace_base_Fork; first apply Htp.
-    eapply ctrace_yield.
-    { rewrite lookup_app_l; last rewrite insert_length -lookup_lt_is_Some //.
-      rewrite list_lookup_insert //. by apply lookup_lt_is_Some. }
-    rewrite insert_app_l; last rewrite insert_length -lookup_lt_is_Some //.
-    rewrite list_insert_insert //.
+  - destruct (is_value e) eqn:Hval.
+    * rewrite /compile_tp in Htr. simpl in Htr. rewrite Hval /= in Htr.
+      exists (CTYield tid' tr).
+      split; first repeat constructor.
+      eapply is_ctrace_insert; first done; first apply compile_Fork_value; first done.
+      simpl.
+      eapply is_ctrace_yield.
+      { rewrite list_lookup_insert //. by apply lookup_lt_is_Some. }
+      rewrite list_insert_insert.
+      rewrite compile_expr_val !bind_ret_l in Htr.
+      by rewrite /= app_nil_r in Htr.
+    * exists (CTFork (compile_expr e ;; kill_thread) (CTYield tid' tr)).
+      split; first repeat constructor.
+      rewrite compile_expr_val !bind_ret_l in Htr.
+      eapply trace_base_Fork; first done; first apply Htp.
+      eapply is_ctrace_yield.
+      { rewrite lookup_app_l; last rewrite insert_length -lookup_lt_is_Some //.
+        rewrite list_lookup_insert //. by apply lookup_lt_is_Some. }
+      rewrite insert_app_l; last rewrite insert_length -lookup_lt_is_Some //.
+      rewrite list_insert_insert //. by rewrite /compile_tp /= Hval /= in Htr.
 Admitted.
 
-Lemma base_step_in_thread_completed {R} e1 σ1 κs e2 σ2 efs tr tid tid' (tp : list (itree heaplangE R)) :
+Lemma base_step_in_thread_completed e1 σ1 κs e2 σ2 efs tr tid tid' (tp : list (itree heaplangE ())) :
   base_step e1 σ1 κs e2 σ2 efs →
   is_value e2 →
-  is_ctrace tr tid' (delete tid tp ++ map (λ e, compile_expr e ;; kill_thread)%itree efs) →
+  is_ctrace tr tid' (delete tid tp ++ compile_tp efs) →
   tp !! tid = Some (compile_expr e1 ;; kill_thread)%itree →
   ∃ tr', is_postfix tr tr' ∧ is_ctrace tr' tid tp.
 Admitted.
 
-Lemma base_step_in_thread_not_completed {R} e1 σ1 κs e2 σ2 efs tr tid tid' (tp : list (itree heaplangE R)) :
+Lemma base_step_in_thread_not_completed e1 σ1 κs e2 σ2 efs tr tid tid' (tp : list (itree heaplangE ())) :
   base_step e1 σ1 κs e2 σ2 efs →
   ~is_value e2 →
-  is_ctrace tr tid' (<[tid:=(compile_expr e2 ;; kill_thread)%itree]>tp ++ map (λ e, compile_expr e ;; kill_thread)%itree efs) →
+  is_ctrace tr tid' (<[tid:=(compile_expr e2 ;; kill_thread)%itree]>tp ++ compile_tp efs) →
   tp !! tid = Some (compile_expr e1 ;; kill_thread)%itree →
   ∃ tr', is_postfix tr tr' ∧ is_ctrace tr' tid tp.
+Admitted.
+
+Lemma base_step_in_thread_last_thread {R} e1 σ1 κs e2 σ2 efs tid :
+  base_step e1 σ1 κs e2 σ2 efs →
+  is_value e2 →
+  Forall is_value efs →
+  ∃ tr, is_ctrace (R := R) tr tid [(compile_expr e1 ;; kill_thread)%itree].
+Admitted.
+
+Lemma base_step_not_value e1 σ1 κs e2 σ2 tfs :
+  base_step e1 σ1 κs e2 σ2 tfs →
+  is_value e1 = false.
+Admitted.
+
+Lemma lt_gt n m :
+  n < m ↔ m > n.
+Admitted.
+
+Lemma fill_is_not_value K e :
+  length K > 0 →
+  is_value (ectx_language.fill K e) = false.
 Admitted.
 
 (* TODO: The idea is to add that if [tp'] has nowhere to step then [tr] ends in
 *        UB, and if [tp'] returns a value, then so does [tr]. *)
+  Search nsteps.
 Lemma has_trace n tp σ tp' σ' κ :
-  nsteps n (tp, σ) κ (tp', σ') →
-  length tp > 0 →
-  ∃ tr i, is_ctrace tr i (map compile_expr (filter unevaluated tp)).
+  language.nsteps n (tp, σ) κ (tp', σ') →
+  length (compile_tp tp) > 0 →
+  ∃ tr tid, is_ctrace (R := ()) tr tid (compile_tp tp).
 Proof.
-  revert tp σ tp' σ' κ. induction n; intros tp σ tp' σ' κ Hstep Hne.
-  { exists CTCut, 0. destruct tp as [|t tp]. { simpl in Hne. lia. }
-    exists (compile_expr t). split; first done. constructor. }
-  inversion Hstep as [|m [tp1 σ1] [tp2 σ2] [tp3 σ3] ? ? Hstep' Hstep'']. subst.
-  inversion Hstep' as [e1 σ1 e2 σ2' efs t1 t2 Htp' Htp2' Hprim].
+  revert tp σ tp' σ' κ. induction n as [|n IH]; intros tp σ tp' σ' κ Hstep Hne.
+  { exists CTCut, 0. apply is_ctrace_CTCut. rewrite map_length.
+    remember (length (List.filter (λ e : expr, negb (is_value e)) tp)).
+    rewrite /compile_tp map_length -Heqn in Hne. lia. }
+  inversion Hstep as [|m [tp1 σ1] [tp2 σ2] [tp3 σ3] ? ? Hstep'' Hstep']. subst.
+  inversion Hstep'' as [e1' σ1 e2' σ2' efs tpa tpb Htp' Htp2' Hprim].
   injection Htp'. intros -> ->. clear Htp'.
   injection Htp2'. intros -> ->. clear Htp2'.
-  inversion Hprim as [K e1' e2' He1 He2 Hbase]. subst. simpl in K, e1', e2'.
-  clear Hstep'' Hstep' Hprim.
-  rewrite map_app /=.
-  setoid_rewrite compile_expr_bind.
+  inversion Hprim as [K e1 e2 He1 He2 Hbase]. subst. simpl in K, e1, e2.
+  clear Hstep'' Hprim.
+  destruct (decide (length K = 0)) as [HK|HK].
+  - apply nil_length_inv in HK as ->. simpl. simpl in *.
+    destruct (is_value e2) eqn:Hval.
+    * destruct (decide (Forall is_value tpa ∧ Forall is_value tpb ∧ Forall is_value efs)) as [[Htp1val [Htp2val Hefsval]]|Hval'].
+      + rewrite compile_tp_app compile_tp_cons !compile_tp_empty // app_nil_l.
+        assert (Hbase' := Hbase). apply base_step_not_value in Hbase' as ->.
+        eapply base_step_in_thread_last_thread with (tid := 0) in Hbase as [tr Htr]; eauto.
+      + apply IH in Hstep' as [tr [tid Htr]]; last first.
+        { rewrite -lt_gt -Nat.neq_0_lt_0. intros Hemp%nil_length_inv.
+          rewrite app_comm_cons !compile_tp_app in Hemp.
+          apply app_eq_nil in Hemp as [Htpa [Htpb Hefs]%app_eq_nil].
+          rewrite compile_tp_cons Hval in Htpb.
+          apply Hval'.
+          split; first by apply compile_tp_empty_inv.
+          split; first by apply compile_tp_empty_inv.
+          by apply compile_tp_empty_inv.
+        }
+        odestruct (base_step_in_thread_completed _ _ _ _ _ _ _ (length (compile_tp tpa)) _ _ Hbase _ _ _) as [tr' [_ Htr']]; eauto; last first.
+        { rewrite compile_tp_app lookup_app_r // Nat.sub_diag compile_tp_cons.
+          assert (Hbase' := Hbase). by apply base_step_not_value in Hbase' as ->. }
+        rewrite compile_tp_app compile_tp_cons.
+        apply base_step_not_value in Hbase as ->.
+        rewrite delete_middle -app_assoc.
+        by rewrite compile_tp_app compile_tp_cons Hval compile_tp_app in Htr.
+      * apply IH in Hstep' as [tr [tid Htr]]; last first.
+        { rewrite -lt_gt -Nat.neq_0_lt_0. intros Hemp%nil_length_inv.
+          rewrite app_comm_cons !compile_tp_app in Hemp.
+          apply app_eq_nil in Hemp as [Htpa [Htpb Hefs]%app_eq_nil].
+          rewrite compile_tp_cons Hval in Htpb.
+          discriminate.
+        }
+        odestruct (base_step_in_thread_not_completed _ _ _ _ _ _ _ (length (compile_tp tpa)) _ _ Hbase _ _ _) as [tr' [_ Htr']]; eauto.
+        1:{ rewrite Hval. eauto. }
+        2:{ rewrite compile_tp_app lookup_app_r // Nat.sub_diag compile_tp_cons.
+          assert (Hbase' := Hbase). by apply base_step_not_value in Hbase' as ->. }
+        rewrite compile_tp_app compile_tp_cons.
+        apply base_step_not_value in Hbase as ->.
+        Search insert length.
+        replace (length (compile_tp tpa)) with (length (compile_tp tpa) + 0) by lia.
+        rewrite insert_app_r /= -app_assoc.
+        by rewrite compile_tp_app compile_tp_cons Hval compile_tp_app in Htr.
+  - apply IH in Hstep' as [tr [tid Htr]]; last first.
+    { rewrite -lt_gt -Nat.neq_0_lt_0. intros Hemp%nil_length_inv.
+      rewrite app_comm_cons !compile_tp_app compile_tp_cons in Hemp.
+      apply app_eq_nil in Hemp as [Htpa [Htpb Hefs]%app_eq_nil].
+      rewrite fill_is_not_value in Htpb; last first. { rewrite -lt_gt -Nat.neq_0_lt_0 //. }
+      discriminate.
+    }
+    rewrite compile_tp_app compile_tp_cons fill_is_not_value  in Htr; last first.
+    { rewrite -lt_gt -Nat.neq_0_lt_0 //. }
+    rewrite compile_expr_bind in Htr; last first.
+    { rewrite -lt_gt -Nat.neq_0_lt_0 //. }
+    { admit. }
+    rewrite compile_tp_app compile_tp_cons fill_is_not_value; last first.
+    { rewrite -lt_gt -Nat.neq_0_lt_0 //. }
+    apply step_in_thread with (tp := (compile_tp tpa ++ (v ← compile_expr e1; yield_if_not_val e1;; compile_expr (fill K (Val v));; kill_thread)%itree :: compile_tp tpb)) (tid := length (compile_tp tpa)) (tid' := tid) (k := λ v, (compile_expr (fill K (Val v));; kill_thread)%itree) (tr := tr) in Hbase as [tr' [_ Htr']].
+    * exists tr'. exists (length (compile_tp tpa)).
+      rewrite compile_expr_bind.
+      + rewrite bind_bind. by setoid_rewrite bind_bind.
+      + admit.
+      + rewrite -lt_gt -Nat.neq_0_lt_0 //.
+    * replace (length (compile_tp tpa)) with (length (compile_tp tpa) + 0) by lia.
+      rewrite compile_tp_app in Htr.
+      rewrite insert_app_r /= -app_assoc /=.
+      rewrite bind_bind in Htr.
+      by setoid_rewrite bind_bind in Htr.
+    * rewrite lookup_app_r // Nat.sub_diag //.
 Admitted.
